successfully derived proxy, derived decOpt over proxy, and tied everything up in terms of the original well_scoped relation

src/Language/PlutusIR/Analysis/WellScoped.v
@@ -1,4 +1,6 @@
 From PlutusCert Require Import
+  Util
+  Util.List
   Language.PlutusIR
   Analysis.BoundVars.
 Import NamedTerm.
@@ -10,6 +12,11 @@ Require Import
 
 Import ListNotations.
 From QuickChick Require Import QuickChick.
+From Sandbox Require Import CTProxy.
+Require Import Coq.Program.Equality.
+
+
+
 
 
 Definition ctx := list string.
@@ -22,7 +29,7 @@ Definition tvd_name (tvd : tvdecl tyname) : tyname :=
 Reserved Notation "Δ '|-*' T" (at level 40, T at level 0).
 Inductive well_scoped_Ty (Δ : ctx) : Ty -> Prop :=
   | WST_Var : forall X,
-      In X Δ ->
+      NameIn X Δ ->
       Δ |-* (Ty_Var X)
   | WST_Fun : forall T1 T2,
       Δ |-* T1 ->
@@ -35,8 +42,8 @@ Inductive well_scoped_Ty (Δ : ctx) : Ty -> Prop :=
   | WST_Forall : forall X K T,
       (X :: Δ) |-* T ->
       Δ |-* (Ty_Forall X K T)
-  | WST_Builtin : forall u,
-      Δ |-* (Ty_Builtin (Some (TypeIn u)))
+  | WST_Builtin : forall u (x : typeIn u),
+      Δ |-* (Ty_Builtin (Some' x))
   | WST_Lam : forall X K1 T,
       (X :: Δ) |-* T ->
       Δ |-* (Ty_Lam X K1 T)
@@ -46,23 +53,50 @@ Inductive well_scoped_Ty (Δ : ctx) : Ty -> Prop :=
       Δ |-* (Ty_App T1 T2) 
 where "Δ '|-*' T " := (well_scoped_Ty Δ T).
 
+QCDerive DecOpt for (well_scoped_Ty Δ ty).
+
+Instance DecOptwell_scoped_Ty_sound Δ ty: DecOptSoundPos (well_scoped_Ty Δ ty).
+Proof. derive_sound. Qed.
+
+
+
+
+
+
 Reserved Notation "Δ ',,' Γ '|-+' t " (at level 101, t at level 0, no associativity).
-Reserved Notation "Δ '|-ok_c' c " (at level 101, c at level 0).
+Reserved Notation "Δ '|-ok_cs' c " (at level 101, c at level 0).
 Reserved Notation "Δ ',,' Γ  '|-oks_nr' bs" (at level 101, bs at level 0, no associativity).
 Reserved Notation "Δ ',,' Γ '|-oks_r' bs" (at level 101, bs at level 0, no associativity).
 Reserved Notation "Δ ',,' Γ '|-ok_b' b" (at level 101, b at level 0, no associativity).
 
-Inductive constructor_well_formed (Δ : ctx) : constructor -> Prop :=
-  | W_Con : forall x T ar,
+Inductive constructors_well_formed (Δ : ctx) : list constructor -> Prop :=
+  | W_Con : forall x T ar cs,
       Δ |-* T ->
-      Δ |-ok_c (Constructor (VarDecl x T) ar)
+      Δ |-ok_cs cs ->
+      Δ |-ok_cs ((Constructor (VarDecl x T) ar) :: cs)
   where 
-    "Δ '|-ok_c' c" := (constructor_well_formed Δ c)
-.
+    "Δ '|-ok_cs' cs" := (constructors_well_formed Δ cs).
+
+QCDerive DecOpt for (constructors_well_formed Δ c).
+
+Instance DecOptconstructors_well_formed_sound Δ c : DecOptSoundPos (constructors_well_formed Δ c).
+Proof. derive_sound. Qed.
+
+
+
+
+
+Definition btvb_app (b : Binding) Δ := btvb b ++ Δ.
+Definition bvb_app (b : Binding) Δ := bvb b ++ Δ.
+Definition map_tvd_name_rev_app x c := rev (map tvd_name x) ++ c.
+Definition rev_btvbs_app (x : list Binding) c := rev (btvbs x) ++ c.
+Definition rev_bvbs_app (x : list Binding) c := rev (bvbs x) ++ c.
+
+Check Forall.
 
 Inductive well_scoped (Δ Γ: ctx) : Term -> Prop :=
   | WS_Var : forall x,
-      In x Γ ->
+      NameIn x Γ ->
       Δ ,, Γ |-+ (Var x)
   | WS_LamAbs : forall x T t,
       Δ |-* T ->
@@ -88,39 +122,35 @@ Inductive well_scoped (Δ Γ: ctx) : Term -> Prop :=
   | WS_Unwrap : forall M,
       Δ ,, Γ |-+ M ->
       Δ ,, Γ |-+ (Unwrap M)
-  | WS_Constant : forall u a,
-      Δ ,, Γ |-+ (Constant (Some (ValueOf u a)))
+  | WS_Constant : forall u (x : valueOf u),
+      Δ ,, Γ |-+ (Constant (Some' x))
   | WS_Builtin : forall f,
       Δ ,, Γ |-+ (Builtin f)
-  | WS_Error : forall S,
-      Δ |-* S ->
-      Δ ,, Γ |-+ (Error S)
+  | WS_Error : forall s,
+      Δ |-* s ->
+      Δ ,, Γ |-+ (Error s)
   | WS_Let : forall bs t Δ' Γ',
-      Δ' = rev (btvbs bs) ++ Δ ->
-      Γ' = rev (bvbs bs) ++ Γ ->
+      Δ' = rev_btvbs_app bs Δ ->
+      Γ' = rev_bvbs_app bs Γ ->
       Δ ,, Γ |-oks_nr bs ->
       Δ' ,, Γ' |-+ t ->
       Δ ,, Γ |-+ (Let NonRec bs t)
   | WS_LetRec : forall bs t Δ' Γ',
-      Δ' = rev (btvbs bs) ++ Δ ->
-      Γ' = rev (bvbs bs) ++ Γ ->
+      Δ' = rev_btvbs_app bs Δ ->
+      Γ' = rev_bvbs_app bs Γ ->
       Δ' ,, Γ' |-oks_r bs ->
       Δ' ,, Γ' |-+ t ->
       Δ ,, Γ |-+ (Let Rec bs t)
-
-
+          
 with bindings_well_formed_nonrec (Δ Γ : ctx) : list Binding -> Prop :=
-
   | W_NilB_NonRec :
-    Δ ,, Γ |-oks_nr nil
-
+      Δ ,, Γ |-oks_nr nil
   | W_ConsB_NonRec : forall b bs,
       Δ ,, Γ |-ok_b b ->
-      (btvb b ++ Δ) ,, (bvb b ++ Γ) |-oks_nr bs ->
+      (btvb_app b Δ) ,, (bvb_app b Γ) |-oks_nr bs ->
       Δ ,, Γ |-oks_nr (b :: bs)
 
 with bindings_well_formed_rec (Δ Γ : ctx) : list Binding -> Prop :=
-
   | W_NilB_Rec :
       Δ ,, Γ |-oks_r nil
   | W_ConsB_Rec : forall b bs,
@@ -137,14 +167,97 @@ with binding_well_formed (Δ Γ : ctx) : Binding -> Prop :=
       Δ |-* T ->
       Δ ,, Γ |-ok_b (TypeBind (TyVarDecl X K) T)
   | W_Data : forall X YKs cs matchFunc Δ',
-      Δ' = rev (map tvd_name YKs) ++ Δ  ->
-      (forall c, In c cs -> Δ' |-ok_c c) ->
+      Δ' = map_tvd_name_rev_app YKs Δ  ->
+      Δ' |-ok_cs cs ->
       Δ ,, Γ |-ok_b (DatatypeBind (Datatype X YKs matchFunc cs))
 
   where "Δ ',,' Γ '|-+' t" := (well_scoped Δ Γ t)
   and "Δ ',,' Γ '|-oks_nr' bs" := (bindings_well_formed_nonrec Δ Γ bs)
   and "Δ ',,' Γ '|-oks_r' bs" := (bindings_well_formed_rec Δ Γ bs)
-  and "Δ ',,' Γ '|-ok_b' b" := (binding_well_formed Δ Γ b)
-.
+  and "Δ ',,' Γ '|-ok_b' b" := (binding_well_formed Δ Γ b).
+          
+
+(* derivation of proxy type *)
+
+MetaCoq Run (deriveCTProxy well_scoped).
+
+
+
+
+(* derivation over proxy type*)
+
+QCDerive DecOpt for (well_scoped_proxy tag).
+
+Instance DecOptwell_scoped_proxy_sound tag : DecOptSoundPos (well_scoped_proxy tag).
+Proof. derive_sound. Qed.
+
+
+
+(* soundness of proxy type over its original definition *)
+
+Theorem well_scoped_proxy_sound : forall tag,
+  well_scoped_proxy tag -> match tag with
+                           | well_scoped_tag c1 c2 tm => well_scoped c1 c2 tm
+                           | bindings_well_formed_nonrec_tag c1 c2 bs => bindings_well_formed_nonrec c1 c2 bs
+                           | bindings_well_formed_rec_tag c1 c2 bs => bindings_well_formed_rec c1 c2 bs
+                           | binding_well_formed_tag c1 c2 b => binding_well_formed c1 c2 b
+                           end.
+Proof with eauto using well_scoped, bindings_well_formed_nonrec, bindings_well_formed_rec, binding_well_formed.
+  intros. dependent induction H; subst...
+Qed.
+
+
+
+(* helper Ltac (is generic, still needs to be given a place) *)
+Ltac derive__sound HCorrect :=
+  unfold DecOptSoundPos;
+  unfold decOpt;
+  intros s H;
+  apply sound in H;
+  apply HCorrect;
+  assumption.
+
+
+
+
+(* well_scoped *)
+
+Instance DecOptwell_scoped c1 c2 tm : DecOpt (well_scoped c1 c2 tm) :=
+{| decOpt s := @decOpt (well_scoped_proxy (well_scoped_tag c1 c2 tm)) (DecOptwell_scoped_proxy (well_scoped_tag c1 c2 tm)) s |}.
+
+Instance DecOptwell_scoped_sound c1 c2 tm : DecOptSoundPos (well_scoped c1 c2 tm).
+Proof. derive__sound (well_scoped_proxy_sound (well_scoped_tag c1 c2 tm)). Qed.
+
+
+
+(* bindings_well_formed_nonrec *)
+
+Instance DecOptbindings_well_formed_nonrec c1 c2 bs : DecOpt (bindings_well_formed_nonrec c1 c2 bs) :=
+{| decOpt s := @decOpt (well_scoped_proxy (bindings_well_formed_nonrec_tag c1 c2 bs)) (DecOptwell_scoped_proxy (bindings_well_formed_nonrec_tag c1 c2 bs)) s |}.
+
+Instance DecOptbindings_bindings_well_formed_nonrec c1 c2 bs : DecOptSoundPos (bindings_well_formed_nonrec c1 c2 bs).
+Proof. derive__sound (well_scoped_proxy_sound (bindings_well_formed_nonrec_tag c1 c2 bs)). Qed.
+
+
+
+(* bindings_well_formed_rec *)
+
+Instance DecOptbindings_well_formed_rec c1 c2 bs : DecOpt (bindings_well_formed_rec c1 c2 bs) :=
+{| decOpt s := @decOpt (well_scoped_proxy (bindings_well_formed_rec_tag c1 c2 bs)) (DecOptwell_scoped_proxy (bindings_well_formed_rec_tag c1 c2 bs)) s |}.
+
+Instance DecOptbindings_bindings_well_formed_rec c1 c2 bs : DecOptSoundPos (bindings_well_formed_rec c1 c2 bs).
+Proof. derive__sound (well_scoped_proxy_sound (bindings_well_formed_rec_tag c1 c2 bs)). Qed.
+
+
+
+(* binding_well_formed *)
+
+Instance DecOptbinding_well_formed c1 c2 bs : DecOpt (binding_well_formed c1 c2 bs) :=
+{| decOpt s := @decOpt (well_scoped_proxy (binding_well_formed_tag c1 c2 bs)) (DecOptwell_scoped_proxy (binding_well_formed_tag c1 c2 bs)) s |}.
+
+Instance DecOptbindings_binding_well_formed c1 c2 b : DecOptSoundPos (binding_well_formed c1 c2 b).
+Proof. derive__sound (well_scoped_proxy_sound (binding_well_formed_tag c1 c2 b)). Qed.
+
+
 
 Definition closed := well_scoped [] [].
